KLR/Semantics/SmallStep.lean
@@ -13,40 +13,39 @@ Each configuration `Prog × State` nondeterministically Steps to anything in the
 We distinguish between error States and terminated States using the `toVal` partial function.
 markusde: Having toVal be a partial function out of Prog × State rather than a total function out of
 { x : Prog × State | stuck x } is more robust against changes to the semantics.
+
+NB: Val and State are `outParams`. All fields involve a Prog term, so this should be unambiguous
+as long as there is at most one `SmallStep` instance per `Prog` type.
 -/
-structure SmallStep : Type _ where
-  /-- The type of Program terms. -/
-  Prog : Type _
-  /-- The type of States. -/
-  State : Type _
-  /-- The type of Values. -/
-  Val : Type _
+class SmallStep (Prog : Type _) (Val State : outParam (Type _)) : Type _ where
   /-- A nondeterministic Stepping relation. -/
   Step : Prog × State → Prog × State → Prop
   /-- Check if a Program is done, and terminate if so. -/
   toVal : Prog → Option Val
   /-- Values must not be able to execute.  -/
-  toVal_isSome_isStuck {p1 p2 : Prog} {s1 s2 : State} : (toVal p1).IsSomeP → Step (p1, s1) (p2, s2) → False
+  toVal_isSome_isStuck {p1 p2 : Prog} {s1 s2 : State} : (toVal p1).isSome → Step (p1, s1) (p2, s2) → False
+export SmallStep (Step toVal toVal_isSome_isStuck)
 
 /-- A small Step semantics is deterministic when every configuration is either stuck,
 or Steps to exactly one State. We also force that the semantics can't take stutter steps, so that
 there is exactly one way that the program can progress at each point. -/
-class Det (S : SmallStep) where
-  step_det {c c'} : S.Step c c' → ∀ c'', S.Step c c'' → c'' = c'
-  step_progress {c c'} : S.Step c c' → c ≠ c'
+class Det (Prog : Type _) (Val State : outParam (Type _)) : Type _ extends SmallStep Prog Val State where
+  step_det {c c'} : Step c c' → ∀ c'', Step c c'' → c'' = c'
+  step_progress {c c'} : Step c c' → c ≠ c'
 export Det (step_det)
+
 
 namespace SmallStep
 
 section basic
-variable (S : SmallStep)
+variable {Prog Val State : Type _} [SmallStep Prog Val State]
 
 /-- A program is a value. -/
-def IsValue (p : S.Prog) : Prop := S.toVal p |>.IsSomeP
+def IsValue (p : Prog) : Prop := toVal p |>.isSome
 
-theorem IsValue_value {p : S.Prog} (H : S.IsValue p) : ∃ v, S.toVal p = some v := by
+theorem IsValue_value {p : Prog} (H : IsValue p) : ∃ v, toVal p = some v := by
   simp_all [IsValue]
-  generalize Hx : S.toVal p = x
+  generalize Hx : toVal p = x
   rw [Hx] at H
   cases x
   · cases H
@@ -55,138 +54,64 @@ theorem IsValue_value {p : S.Prog} (H : S.IsValue p) : ∃ v, S.toVal p = some v
     exists v
 
 /-- A configuration is stuck. -/
-def IsStuck (c : S.Prog × S.State) : Prop := ∀ {c'}, S.Step c c' → False
+def IsStuck (c : Prog × State) : Prop := ∀ {c'}, Step c c' → False
 
 /-- N-step stepping relation. -/
-inductive StepN : Nat → S.Prog × S.State → S.Prog × S.State → Prop where
+inductive StepN : Nat → Prog × State → Prog × State → Prop where
 | done : c = c' → StepN 0 c c'
-| step : S.Step c c' → StepN n c' c'' → StepN n.succ c c''
+| step : Step c c' → StepN n c' c'' → StepN n.succ c c''
 
 /-- Demonic nontermination: There is no terminating trace.
 This is stronger than the usual definition of nontermination, but is easy to work with
 and equivalent to in the deterministic case. -/
-def Nonterminating (c : S.Prog × S.State) : Prop :=
-  ∀ {n c'}, S.StepN n c c' → ¬ S.IsStuck c'
+def Nonterminating (c : Prog × State) : Prop :=
+  ∀ {n c'}, StepN n c c' → ¬ IsStuck c'
 
 /-- Angelic termination: There exists a terminating trace. -/
-def MayTerminate (c : S.Prog × S.State) : Prop :=
-  ∃ n c', S.StepN n c c' ∧ S.IsStuck c'
+def MayTerminate (c : Prog × State) : Prop :=
+  ∃ n c', StepN n c c' ∧ IsStuck c'
 
 /-- Demonic termination: there exists N such that it is not possible for any trace to take
 more than N steps. -/
-def Terminating (c : S.Prog × S.State) : Prop :=
-  ∃ N, ∀ c' N', N < N' → ¬S.StepN N' c c'
+def Terminating (c : Prog × State) : Prop :=
+  ∃ N, ∀ c' N', N < N' → ¬StepN N' c c'
 
 /-- There is exactly one state that the program can terminate in. -/
-def UniquelyTerminating (c : S.Prog × S.State) : Prop :=
-  ∃ N c', (S.StepN N c c') ∧ (S.IsStuck c') ∧ (∀ N'  c'', S.StepN N' c c'' → S.IsStuck c'' → N = N' ∧ c' = c'')
+def UniquelyTerminating (c : Prog × State) : Prop :=
+  ∃ N c', (StepN N c c') ∧ (IsStuck c') ∧ (∀ N'  c'', StepN N' c c'' → IsStuck c'' → N = N' ∧ c' = c'')
 
 /-- All finite traces of a configuration only ever get stuck in value states. -/
-def Safe {S : SmallStep} (c : S.Prog × S.State) : Prop :=
-  ∀ {n p s}, S.StepN n c (p, s) → S.IsStuck (p, s) → S.IsValue p
+def Safe  (c : Prog × State) : Prop :=
+  ∀ {n p s}, StepN n c (p, s) → IsStuck (p, s) → IsValue p
 
-theorem stepN_zero_inv (H : S.StepN 0 c c') : c = c' := by
+theorem stepN_zero_inv {c c' : Prog × State} (H : StepN 0 c c') : c = c' := by
   rcases H with ⟨rfl⟩|_; rfl
 
-theorem step_of_stepN_one (H : S.StepN 1 c c') : S.Step c c' := by
+theorem step_of_stepN_one {c c' : Prog × State} (H : StepN 1 c c') : Step c c' := by
   rcases H with _|⟨H, rfl|_⟩; exact H
 
-theorem stepN_isStuck_inv (H : S.StepN m c c') (Hs : S.IsStuck c) : m = 0 := by
+theorem stepN_isStuck_inv {c c' : Prog × State} (H : StepN m c c') (Hs : IsStuck c) : m = 0 := by
   rcases H with _|H
   · rfl
   · exact False.elim (Hs H)
 
-theorem stepN_1_iff_step : S.StepN 1 c1 c2 ↔ S.Step c1 c2 := by
+theorem stepN_1_iff_step {c1 c2 : Prog × State} : StepN 1 c1 c2 ↔ Step c1 c2 := by
   refine ⟨?_, (StepN.step · (StepN.done rfl))⟩
   rintro (_|⟨H,He|_⟩)
   exact He▸H
 
-theorem step_not_isStuck : S.Step (p1, s1) (p1', s1') → ¬(S.IsStuck (p1, s1)) :=
+theorem step_not_isStuck {p1 p1' : Prog} {s1 s1' : State} : Step (p1, s1) (p1', s1') → ¬(IsStuck (p1, s1)) :=
   (· |> ·)
 
 /-- For all programs, they either map teminate, or they don't. -/
-theorem weak_termination_em c : S.MayTerminate c ∨ S.Nonterminating c := by
-  if Hem : S.Nonterminating c then exact .inr Hem else
+theorem weak_termination_em {c : Prog × State} : MayTerminate c ∨ Nonterminating c := by
+  if Hem : Nonterminating c then exact .inr Hem else
   refine (.inl ?_)
   simp only [Nonterminating, Prod.forall, Classical.not_forall, not_imp, Classical.not_not] at Hem
   rcases Hem with ⟨n, p, s, _, _⟩; exists n; exists (p, s)
 
-end basic
-
-section det
-
-
-variable {S : SmallStep} [Det S]
-
--- TODO: Cleanup
-theorem stepN_detN {n1 n2 c'} : ∀ {c}, S.IsStuck c' → S.StepN n1 c c' → S.StepN n2 c c' → n1 = n2 := by
-  intros _ _ H1
-  induction H1 generalizing n2
-  · intro H2
-    rename_i H Hs
-    exact (S.stepN_isStuck_inv H2 (H ▸ Hs)).symm
-  · rename_i n c'' Hs Hsn IH Ht
-    intro Hsn'
-    cases n2
-    · exfalso
-      have H'' := S.stepN_zero_inv Hsn'; subst H''
-      apply Ht Hs
-    rename_i n2
-    congr
-    apply IH Ht
-    cases Hsn'
-    rename_i c'' Hs' Hsn'
-    have Hx := step_det Hs _ Hs'
-    exact Hx ▸ Hsn'
-
--- TODO: Cleanup
-theorem stepN_det {n1 n2 c1 c2} (Hs : S.IsStuck c1) (Hs2 : S.IsStuck c2):
-    ∀ {c}, S.StepN n1 c c1 → S.StepN n2 c c2 → n1 = n2 ∧ c1 = c2 := by
-  revert c2 n2
-  induction n1
-  · intro n2 c2 Hs2 c Hcc1 Hcc2
-    have Hcc1' := S.stepN_zero_inv Hcc1 <;> subst Hcc1'
-    cases n2
-    · have Hcc2' := S.stepN_zero_inv Hcc2 <;> subst Hcc2'
-      exact ⟨rfl, rfl⟩
-    · -- c = c1 and c1 is stuck
-      rename_i n; exfalso
-      cases Hcc2
-      rename_i _ Hstep _
-      apply Hs
-      apply Hstep
-  · rename_i n1 IH
-    intro n2 c2 Hs2 c HstepN1 HStepN2
-    cases HstepN1
-    rename_i c1' Hcc1' Hc'c1
-    cases n2
-    · exfalso
-      -- c = c2
-      have Hcc2' := S.stepN_zero_inv HStepN2
-      clear HStepN2
-      apply (Hcc2' ▸ Hs2) Hcc1'
-    rename_i n2
-    simp
-    apply IH
-    · apply Hs2
-    · apply Hc'c1
-    cases HStepN2
-    rename_i H1 H2 H3
-    rw [← step_det Hcc1' _ H2]
-    trivial
-
-/-- For determinisic programs, if it might terminate, then it is uniquely terminating -/
-theorem uniquelyTerminating_of_mayTerinate c : S.MayTerminate c → S.UniquelyTerminating c := by
-  rintro ⟨N, c', Hs, Ht⟩; exact ⟨N, c', Hs, Ht, fun N' c'' Hs' Ht' => stepN_det Ht Ht' Hs Hs'⟩
-
-/-- All deterministic programs either terminate, or they don't -/
-theorem uniquelyTerminating_em c : S.UniquelyTerminating c ∨ S.Nonterminating c :=
-  (S.weak_termination_em c).elim (.inl ∘ uniquelyTerminating_of_mayTerinate _) .inr
-
-end det
-
-theorem StepN_add_iff {S : SmallStep} {n1 n2 : Nat} {c1 c2} :
-    S.StepN (n1 + n2) c1 c2 ↔ ∃ c3, S.StepN n1 c1 c3 ∧ S.StepN n2 c3 c2 := by
+theorem StepN_add_iff {n1 n2 : Nat} {c1 c2 : Prog × State} :
+    StepN (n1 + n2) c1 c2 ↔ ∃ c3, StepN n1 c1 c3 ∧ StepN n2 c3 c2 := by
   revert n2 c1 c2
   induction n1
   · intro n2 c1 c2
@@ -218,64 +143,138 @@ theorem StepN_add_iff {S : SmallStep} {n1 n2 : Nat} {c1 c2} :
       apply IH.mpr
       exists c3
 
-theorem stepN_eq [Det S] {n c c1 c2} : S.StepN n c c1 → S.StepN n c c2 → c1 = c2 := by
+/-- A program steps to a value in exactly n steps -/
+def StepsToValue  (n : Nat) (c : Prog × State) (v : Val) :=
+  ∃ c', StepN n c c' ∧ toVal c'.1 = some v
+
+/-- A program takes at least n steps -/
+def StepsAtLeast  (n : Nat) (c : Prog × State) :=
+  ∃ c', StepN n c c'
+
+theorem StepsAtLeast_zero {c : Prog × State} : StepsAtLeast 0 c :=
+  ⟨c, StepN.done rfl⟩
+
+
+end basic
+
+section det
+
+variable {Prog Val State : Type _} [Det Prog Val State]
+
+-- TODO: Cleanup
+theorem stepN_detN {n1 n2} {c' : Prog × State} : ∀ {c}, IsStuck c' → StepN n1 c c' → StepN n2 c c' → n1 = n2 := by
+  intros _ _ H1
+  induction H1 generalizing n2
+  · intro H2
+    rename_i H Hs
+    exact (stepN_isStuck_inv H2 (H ▸ Hs)).symm
+  · rename_i n c'' Hs Hsn IH Ht
+    intro Hsn'
+    cases n2
+    · exfalso
+      have H'' := stepN_zero_inv Hsn'; subst H''
+      apply Ht Hs
+    rename_i n2
+    congr
+    apply IH Ht
+    cases Hsn'
+    rename_i c'' Hs' Hsn'
+    have Hx := step_det Hs _ Hs'
+    exact Hx ▸ Hsn'
+
+-- TODO: Cleanup
+theorem stepN_det {n1 n2} {c1 c2 : Prog × State} (Hs : IsStuck c1) (Hs2 : IsStuck c2):
+    ∀ {c}, StepN n1 c c1 → StepN n2 c c2 → n1 = n2 ∧ c1 = c2 := by
+  revert c2 n2
+  induction n1
+  · intro n2 c2 Hs2 c Hcc1 Hcc2
+    have Hcc1' := stepN_zero_inv Hcc1 <;> subst Hcc1'
+    cases n2
+    · have Hcc2' := stepN_zero_inv Hcc2 <;> subst Hcc2'
+      exact ⟨rfl, rfl⟩
+    · -- c = c1 and c1 is stuck
+      rename_i n; exfalso
+      cases Hcc2
+      rename_i _ Hstep _
+      apply Hs
+      apply Hstep
+  · rename_i n1 IH
+    intro n2 c2 Hs2 c HstepN1 HStepN2
+    cases HstepN1
+    rename_i c1' Hcc1' Hc'c1
+    cases n2
+    · exfalso
+      -- c = c2
+      have Hcc2' := stepN_zero_inv HStepN2
+      clear HStepN2
+      apply (Hcc2' ▸ Hs2) Hcc1'
+    rename_i n2
+    simp
+    apply IH
+    · apply Hs2
+    · apply Hc'c1
+    cases HStepN2
+    rename_i H1 H2 H3
+    rw [← step_det Hcc1' _ H2]
+    trivial
+
+/-- For determinisic programs, if it might terminate, then it is uniquely terminating -/
+theorem uniquelyTerminating_of_mayTerinate {c : Prog × State} : MayTerminate c → UniquelyTerminating c := by
+  rintro ⟨N, c', Hs, Ht⟩; exact ⟨N, c', Hs, Ht, fun N' c'' Hs' Ht' => stepN_det Ht Ht' Hs Hs'⟩
+
+/-- All deterministic programs either terminate, or they don't -/
+theorem uniquelyTerminating_em (c : Prog × State) : UniquelyTerminating c ∨ Nonterminating c :=
+  (weak_termination_em (c := c)).elim (fun c' => .inl <| uniquelyTerminating_of_mayTerinate c') .inr
+
+
+theorem stepN_eq  {n} {c c1 c2 : Prog × State} : StepN n c c1 → StepN n c c2 → c1 = c2 := by
   revert c
   induction n with | zero => ?_ | succ n IH => ?_
-  · intro _ H1 H2; rw [← S.stepN_zero_inv H1, ← S.stepN_zero_inv H2]
+  · intro _ H1 H2; rw [← stepN_zero_inv H1, ← stepN_zero_inv H2]
   · intro c H1 H2
     rw [Nat.add_comm] at H1 H2
     obtain ⟨c1', Hc1', H1⟩ := StepN_add_iff.mp H1
     obtain ⟨c2', Hc2', H2⟩ := StepN_add_iff.mp H2
-    obtain rfl : c1' = c2' := Det.step_det (S.step_of_stepN_one Hc2') _ (S.step_of_stepN_one Hc1')
+    obtain rfl : c1' = c2' := Det.step_det (step_of_stepN_one Hc2') _ (step_of_stepN_one Hc1')
     exact IH H1 H2
 
-theorem Nonterminating_step [Det S] {c : S.Prog × S.State} (H : S.Nonterminating c) :
-    ∃ c', S.Step c c' := by
-  if h : S.IsStuck c
+theorem Nonterminating_step {c : Prog × State} (H : Nonterminating c) :
+    ∃ c', Step c c' := by
+  if h : IsStuck c
     then exact H (.done rfl) h |>.elim
     else exact Classical.not_forall_not.mp h
 
-theorem Nonterminating_step_Nonterminating [Det S] {c : S.Prog × S.State} (H : S.Nonterminating c) (Hs : S.Step c c'):
-    S.Nonterminating c' := fun HS HK' => (H (.step Hs HS) HK').elim
+theorem Nonterminating_step_Nonterminating {c : Prog × State} (H : Nonterminating c) (Hs : Step c c'):
+    Nonterminating c' := fun HS HK' => (H (.step Hs HS) HK').elim
 
-/-- A program steps to a value in exactly n steps -/
-def StepsToValue {S : SmallStep} (n : Nat) (c : S.Prog × S.State) (v : S.Val) :=
-  ∃ c', S.StepN n c c' ∧ S.toVal c'.1 = some v
 
-/-- A program takes at least n steps -/
-def StepsAtLeast {S : SmallStep} (n : Nat) (c : S.Prog × S.State) :=
-  ∃ c', S.StepN n c c'
-
-theorem StepsAtLeast_zero {S : SmallStep} {c : S.Prog × S.State} : S.StepsAtLeast 0 c :=
-  ⟨c, StepN.done rfl⟩
-
-theorem StepsAtLeast_succ [Det S] {c c' : S.Prog × S.State} (Hs : S.Step c c') (H : S.StepsAtLeast n c') :
-    S.StepsAtLeast (n + 1) c := by
+theorem StepsAtLeast_succ {c c' : Prog × State} (Hs : Step c c') (H : StepsAtLeast n c') :
+    StepsAtLeast (n + 1) c := by
   rcases H with ⟨c'', Hc''⟩
   exists c''
   rw [Nat.add_comm, StepN_add_iff]
-  exact ⟨c', ⟨S.stepN_1_iff_step.mpr Hs, Hc''⟩⟩
+  exact ⟨c', ⟨stepN_1_iff_step.mpr Hs, Hc''⟩⟩
 
-theorem Nonterminating_StepsAtLeast [Det S] {c : S.Prog × S.State} (H : S.Nonterminating c) :
-    S.StepsAtLeast n c := by
+theorem Nonterminating_StepsAtLeast {c : Prog × State} (H : Nonterminating c) :
+    StepsAtLeast n c := by
   revert c
   induction n with | zero => exact fun {c} H => StepsAtLeast_zero | succ n IH => ?_
   intro c H
   rcases (Nonterminating_step H) with ⟨c', Hstep_c'⟩
   exact StepsAtLeast_succ Hstep_c' (IH <| Nonterminating_step_Nonterminating H Hstep_c')
 
-theorem Nonterminating_not_StepsToValue [Det S] {c : S.Prog × S.State} {n : Nat} {v : S.Val}
-    (Hn : S.Nonterminating c) (H : S.StepsToValue n c v) : False := by
-  obtain ⟨cf, Hk⟩ := @S.Nonterminating_StepsAtLeast (n + 1) _ _ Hn
+theorem Nonterminating_not_StepsToValue {c : Prog × State} {n : Nat} {v : Val}
+    (Hn : Nonterminating c) (H : StepsToValue n c v) : False := by
+  obtain ⟨cf, Hk⟩ := @Nonterminating_StepsAtLeast _ _ _ _ (n + 1) _ Hn -- (n + 1) _ _ Hn
   rw [StepN_add_iff] at Hk; rcases Hk with ⟨cf', H1, H2⟩
   obtain ⟨cf'', H3, H4⟩ := H
   obtain rfl := stepN_eq H1 H3
-  apply @S.toVal_isSome_isStuck cf'.1 cf.1 cf'.2 cf.2
-  · rw [H4]; exact Option.IsSomeP.some
-  · exact S.stepN_1_iff_step.mp H2
+  apply @toVal_isSome_isStuck _ _ _ _ cf'.1 cf.1 cf'.2 cf.2
+  · rw [H4]; simp
+  · exact stepN_1_iff_step.mp H2
 
-theorem stepN_isStuck_stepAtLeast_le [Det S] {n1 n2 : Nat} {c c' : S.Prog × S.State}
-    (Hs : S.StepN n1 c c') (Hst : S.IsStuck c') (HL : S.StepsAtLeast n2 c) : n2 ≤ n1 := by
+theorem stepN_isStuck_stepAtLeast_le {n1 n2 : Nat} {c c' : Prog × State}
+    (Hs : StepN n1 c c') (Hst : IsStuck c') (HL : StepsAtLeast n2 c) : n2 ≤ n1 := by
   false_or_by_contra; rename_i HK
   have HR : n2 = n1 + ((n2 - n1 - 1) + 1) := by omega
   rw [HR] at HL
@@ -286,43 +285,64 @@ theorem stepN_isStuck_stepAtLeast_le [Det S] {n1 n2 : Nat} {c c' : S.Prog × S.S
   obtain rfl : c' = c3 := stepN_eq Hs Hc3
   rw [Nat.add_comm, StepN_add_iff] at H4
   rcases H4 with ⟨_, HK, _⟩
-  exact Hst (S.step_of_stepN_one HK)
+  exact Hst (step_of_stepN_one HK)
 
-theorem stepN_isStuck_stepAtLeast_false [Det S] {n1 n2 : Nat} {c c' : S.Prog × S.State}
-    (Hs : S.StepN n1 c c') (Hst : S.IsStuck c') (HL : S.StepsAtLeast n2 c) : n1 < n2 → False := by
+theorem stepN_isStuck_stepAtLeast_false {n1 n2 : Nat} {c c' : Prog × State}
+    (Hs : StepN n1 c c') (Hst : IsStuck c') (HL : StepsAtLeast n2 c) : n1 < n2 → False := by
   have _ := stepN_isStuck_stepAtLeast_le Hs Hst HL; omega
+
+end det
+
+
+section equivdefs
+
+
+variable {Prog Val State : Type _} [SmallStep Prog Val State]
 
 /-- Program equivalence.
 
 Two programs are equivlent when they are equiterminating,
 and if they terminate, they terminate in values, that are related by Φf.
 -/
-def PRel {S : SmallStep} (c1 c2 : S.Prog × S.State) (Φf : S.Val → S.Val → Prop) : Prop :=
-  (∃ n1 n2 v1 v2, S.StepsToValue n1 c1 v1 ∧ S.StepsToValue n2 c2 v2 ∧ Φf v1 v2) ∨
-  (S.Nonterminating c1 ∧ S.Nonterminating c2)
+def PRel (c1 c2 : Prog × State) (Φf : Val → Val → Prop) : Prop :=
+  (∃ n1 n2 v1 v2, StepsToValue n1 c1 v1 ∧ StepsToValue n2 c2 v2 ∧ Φf v1 v2) ∨
+  (Nonterminating c1 ∧ Nonterminating c2)
 
 /-- Bounded stuttering -/
-def PRelN {S : SmallStep} (n K : Nat) (c1 c2 : S.Prog × S.State) (Φf : S.Val → S.Val → Prop) : Prop :=
-  (∃ n1 n2 v1 v2, n1 ≤ (n * K) ∧ n2 ≤ (n * K) ∧ S.StepsToValue n1 c1 v1 ∧ S.StepsToValue n2 c2 v2 ∧ Φf v1 v2) ∨
-  (S.StepsAtLeast n c1 ∧ S.StepsAtLeast n c2)
+def PRelN (n K : Nat) (c1 c2 : Prog × State) (Φf : Val → Val → Prop) : Prop :=
+  (∃ n1 n2 v1 v2, n1 ≤ (n * K) ∧ n2 ≤ (n * K) ∧ StepsToValue n1 c1 v1 ∧ StepsToValue n2 c2 v2 ∧ Φf v1 v2) ∨
+  (StepsAtLeast n c1 ∧ StepsAtLeast n c2)
 
--- Note: Instead of saying it stutter steps to a value, we can just condition on if it's a value
--- already. Simplifies our lives for nontrivial programs because if it's not a value we can just add
--- another stutter step in between.
-
-def PRelS {S : SmallStep} (n K : Nat) (c1 c2 : S.Prog × S.State) (Φf : S.Val → S.Val → Prop) : Prop :=
+def PRelS (n K : Nat) (c1 c2 : Prog × State) (Φf : Val → Val → Prop) : Prop :=
   match n with
   | .zero => True
   | .succ n' =>
-      match S.toVal c1.1, S.toVal c2.1 with
+      match toVal c1.1, toVal c2.1 with
       | some v1, some v2 => Φf v1 v2
       | _, _ => ∃ n1 n2 c1' c2',
         0 < n1 ∧ 0 < n2 ∧ n1 ≤ K ∧ n2 ≤ K ∧
-        S.StepN n1 c1 c1' ∧ S.StepN n2 c2 c2' ∧ S.PRelS n' K c1' c2' Φf
+        StepN n1 c1 c1' ∧ StepN n2 c2 c2' ∧ PRelS n' K c1' c2' Φf
+
+
+-- TODO: Transitivity of PRel
+
+theorem PRelS.mono_Φ {c1 c2 : Prog × State} {Φf1 Φf2: Val → Val → Prop}
+  (Hmono : ∀ v1 v2, Φf1 v1 v2 → Φf2 v1 v2) : PRelS n K c1 c2 Φf1 → PRelS n K c1 c2 Φf2 := sorry
+
+theorem PRelS.mono_K {c1 c2 : Prog × State} {Φf1 Φf2: Val → Val → Prop}
+  (Hmono : K' ≤ K) : PRelS n K' c1 c2 Φf1 → PRelS n K c1 c2 Φf2 := sorry
+
+end equivdefs
+
+
+
+section equivlimit
+
+variable {Prog Val State : Type _} [Det Prog Val State]
 
 /-- PRel is approximated by PRelN for any stuttering bound -/
-theorem PrelNLimit [Det S] (K : Nat) {c1 c2 : S.Prog × S.State} {Φf : S.Val → S.Val → Prop} :
-    (∀ n, S.PRelN n K c1 c2 Φf) → S.PRel c1 c2 Φf := by
+theorem PrelNLimit (K : Nat) {c1 c2 : Prog × State} {Φf : Val → Val → Prop} :
+    (∀ n, PRelN n K c1 c2 Φf) → PRel c1 c2 Φf := by
   intro Hrel
   rcases (uniquelyTerminating_em c1) with (⟨n1, c1', HStep1, HStuck1, Hut1⟩|H1) <;>
   rcases (uniquelyTerminating_em c2) with (⟨n2, c2', HStep2, HStuck2, Hut2⟩|H2)
@@ -331,70 +351,29 @@ theorem PrelNLimit [Det S] (K : Nat) {c1 c2 : S.Prog × S.State} {Φf : S.Val �
       rcases H with ⟨n1', n2', v1', v2', _, _, _, _, _⟩
       exists n1'; exists n2'; exists v1'; exists v2'
     · exfalso
-      apply S.stepN_isStuck_stepAtLeast_false HStep2 HStuck2 H.2
+      apply stepN_isStuck_stepAtLeast_false HStep2 HStuck2 H.2
       omega
   · rcases Hrel (n1 + 1) with (H|H)  <;> exfalso
     · rcases H with ⟨_, _, _, _, _, _, _, HK, _⟩
-      exact S.Nonterminating_not_StepsToValue H2 HK
-    · exact S.stepN_isStuck_stepAtLeast_false HStep1 HStuck1 H.1 n1.lt_add_one
+      exact Nonterminating_not_StepsToValue H2 HK
+    · exact stepN_isStuck_stepAtLeast_false HStep1 HStuck1 H.1 n1.lt_add_one
   · rcases Hrel (n2 + 1) with (H|H)  <;> exfalso
     ·  -- Can't be the case, because c1 steps to a value but is also nonterminating
       rcases H with ⟨_, _, _, _, _, _, HK, _⟩
-      exact S.Nonterminating_not_StepsToValue H1 HK
-    · apply S.stepN_isStuck_stepAtLeast_false HStep2 HStuck2 H.2
+      exact Nonterminating_not_StepsToValue H1 HK
+    · apply stepN_isStuck_stepAtLeast_false HStep2 HStuck2 H.2
       exact n2.lt_add_one
   · exact .inr ⟨H1, H2⟩
 
-
-/-
-theorem PRelS_trivial_core [Det S] {c1 c2 c1' c2' : S.Prog × S.State} {Φf : S.Val → S.Val → Prop} {n : Nat} :
-    S.StepN n c1 c1' → S.StepN n c2 c2' → S.PRelS n c1 c2 Φf := by
-  revert c1 c2 c1' c2'
-  induction n; simp [PRelS]
-  rename_i n' IH
-  intro c1 c2 c1' c2' H1 H2
-  simp only [PRelS]
-  right
-  obtain ⟨c1'', H1', HR1⟩ := S.StepN_add_iff.mp (Nat.add_comm _ _ ▸ H1)
-  obtain ⟨c2'', H2', HR2⟩ := S.StepN_add_iff.mp (Nat.add_comm _ _ ▸ H2)
-  exists 0
-  exists 0
-  exists c1''
-  exists c2''
-  refine ⟨H1', H2', IH HR1 HR2⟩
--/
-
-/-
-theorem PRelS_trivial [Det S] {c1 c2 c1' c2' : S.Prog × S.State} {Φf : S.Val → S.Val → Prop} {n nl nr : Nat} :
-    S.StepN nl c1 c1' → S.StepN nr c2 c2' → n ≤ nl → n ≤ nr → S.PRelS n c1 c2 Φf := by
-  revert c1 c2 c1' c2' nl nr
-  induction n; simp [PRelS]
-  -- rename_i n' IH
-  -- intro c1 c2 c1' c2' nl nr H1 H2 Hnl Hnr
-  -- simp only [PRelS]
-  sorry
-  -- right
-  -- rcases nl with (_|nl); omega
-  -- rcases nr with (_|nr); omega
-  -- obtain ⟨c1'', H1', HR1⟩ := S.StepN_add_iff.mp (Nat.add_comm _ _ ▸ H1)
-  -- obtain ⟨c2'', H2', HR2⟩ := S.StepN_add_iff.mp (Nat.add_comm _ _ ▸ H2)
-  -- exists 0
-  -- exists 0
-  -- exists c1''
-  -- exists c2''
-  -- refine ⟨H1', H2', ?_⟩
-  -- exact IH HR1 HR2 (Nat.le_of_lt_succ Hnl) (Nat.le_of_lt_succ Hnr)
--/
-
 /-- PRelN is equivalent to the recursive version PRelS -/
-theorem PRelNS [Det S] {c1 c2 : S.Prog × S.State} {Φf : S.Val → S.Val → Prop} (n : Nat) :
-    S.PRelS n K c1 c2 Φf → S.PRelN n K c1 c2 Φf := by
+theorem PRelNS {c1 c2 : Prog × State} {Φf : Val → Val → Prop} (n : Nat) :
+    PRelS n K c1 c2 Φf → PRelN n K c1 c2 Φf := by
   revert c1 c2
   induction n with | zero => ?_ | succ n IH => ?_
   · exact fun _ => .inr ⟨StepsAtLeast_zero, StepsAtLeast_zero⟩
   intro c1 c2 HrelS
   simp only [PRelS] at HrelS
-  cases H1 : S.toVal c1.fst <;> cases H2 : S.toVal c2.fst <;> simp only [H1, H2] at HrelS
+  cases H1 : toVal c1.fst <;> cases H2 : toVal c2.fst <;> simp only [H1, H2] at HrelS
   · -- Neither are values, they both take between 1 and K steps.
     rcases HrelS with ⟨n1, n2, c1', c2', Hpos1, Hpos2, Hn1K, Hn2K, Hc1c1', Hc2c2', Hrec⟩
     rcases IH Hrec with (H|H)
@@ -422,8 +401,8 @@ theorem PRelNS [Det S] {c1 c2 : S.Prog × S.State} {Φf : S.Val → S.Val → Pr
       exact HΦ
     · right
       rcases H with ⟨⟨z1,Hz1⟩,⟨z2,Hz2⟩⟩
-      have HFL : S.StepN (n1 + n) c1 z1 := by apply StepN_add_iff.mpr; exists c1'
-      have HFR : S.StepN (n2 + n) c2 z2 := by apply StepN_add_iff.mpr; exists c2'
+      have HFL : StepN (n1 + n) c1 z1 := by apply StepN_add_iff.mpr; exists c1'
+      have HFR : StepN (n2 + n) c2 z2 := by apply StepN_add_iff.mpr; exists c2'
       rcases n1 with (_|n1); omega
       rcases n2 with (_|n2); omega
       obtain X : n1 + 1 + n = n + 1 + n1 := by omega
@@ -439,16 +418,16 @@ theorem PRelNS [Det S] {c1 c2 : S.Prog × S.State} {Φf : S.Val → S.Val → Pr
     rcases HrelS with ⟨_, nk, _, _, _, _, _, _, _, HK, _⟩
     cases nk; omega
     obtain ⟨z, HK1, _⟩ := StepN_add_iff.mp (Nat.add_comm _ _ ▸ HK)
-    apply @S.toVal_isSome_isStuck c2.1 z.1 c2.2 z.2
-    · rw [H2]; exact Option.IsSomeP.some
-    · exact S.stepN_1_iff_step.mp HK1
+    apply @toVal_isSome_isStuck _ _ _ _ c2.1 z.1 c2.2 z.2
+    · rw [H2]; simp
+    · exact stepN_1_iff_step.mp HK1
   · exfalso
     rcases HrelS with ⟨nk, _, _, _, _, _, _, _, HK, _⟩
     cases nk; omega
     obtain ⟨z, HK1, _⟩ := StepN_add_iff.mp (Nat.add_comm _ _ ▸ HK)
-    apply @S.toVal_isSome_isStuck c1.1 z.1 c1.2 z.2
-    · rw [H1]; exact Option.IsSomeP.some
-    · exact S.stepN_1_iff_step.mp HK1
+    apply @toVal_isSome_isStuck _ _ _ _ c1.1 z.1 c1.2 z.2
+    · rw [H1]; simp
+    · exact stepN_1_iff_step.mp HK1
   · left
     rename_i v1 v2
     exists 0; exists 0; exists v1; exists v2
@@ -458,16 +437,11 @@ theorem PRelNS [Det S] {c1 c2 : S.Prog × S.State} {Φf : S.Val → S.Val → Pr
     refine ⟨⟨c2, StepN.done rfl, H2⟩, ?_⟩
     exact HrelS
 
-theorem PRelS.mono_Φ {S : SmallStep} {c1 c2 : S.Prog × S.State} {Φf1 Φf2: S.Val → S.Val → Prop}
-  (Hmono : ∀ v1 v2, Φf1 v1 v2 → Φf2 v1 v2) : PRelS n K c1 c2 Φf1 → PRelS n K c1 c2 Φf2 := sorry
-
-theorem PRelS.mono_K {S : SmallStep} {c1 c2 : S.Prog × S.State} {Φf1 Φf2: S.Val → S.Val → Prop}
-  (Hmono : K' ≤ K) : PRelS n K' c1 c2 Φf1 → PRelS n K c1 c2 Φf2 := sorry
 
 /-- Unary safety property as a relational property.
 If PRelS holds between a program and itself, then the program is safe. -/
-theorem Safe_of_PRel [Det S] {c : S.Prog × S.State} {Φf : S.Val → S.Val → Prop} :
-    S.PRel c c Φf → S.Safe c := by
+theorem Safe_of_PRel {c : Prog × State} {Φf : Val → Val → Prop} :
+    PRel c c Φf → Safe c := by
   intro H
   rcases H with (⟨n1,n2,v1,v2,Hs1,Hs2,HΦ⟩|H)
   · intro n' p' s' Hn' Hp's'
@@ -476,10 +450,13 @@ theorem Safe_of_PRel [Det S] {c : S.Prog × S.State} {Φf : S.Val → S.Val → 
       unfold IsValue
       rw [this, Hcv]
       constructor
-    have ⟨H1, H2⟩ := @S.stepN_det _ n1 n' cv (p', s') ?G Hp's' c Hstcv Hn'
+    have ⟨H1, H2⟩ := @stepN_det _ _ _ _ n1 n' cv (p', s') ?G Hp's' c Hstcv Hn'
     case G =>
       intro cK HK
-      exact (S.toVal_isSome_isStuck (Option.isSomeP_iff_isSome.mpr (by rw [Hcv]; constructor)) HK).elim
+      apply (toVal_isSome_isStuck ?_ HK).elim
+      exact Option.isSome_of_mem Hcv
     rw [H2]
   · intro n' p' s' Hn' Hp's'
     exact (H.1 Hn' Hp's').elim
+
+end equivlimit
